books/projects/x86isa/machine/decoding-and-spec-utils.lisp
@@ -2212,3 +2212,5 @@ reference made from privilege level 3.</blockquote>"
            (the (signed-byte #.*max-linear-address-size*) start-rip))))
     (and (> length 15)
          length)))
+
+;; ======================================================================
