books/projects/x86isa/portcullis/sharp-dot-constants.lisp
@@ -82,6 +82,8 @@
 (defconst *2^64-1*    (- *2^64* 1))
 (defconst *2^127*     (expt 2 127))
 (defconst *2^128*     (expt 2 128))
+(defconst *2^256*     (expt 2 256))
+(defconst *2^512*     (expt 2 512))
 (defconst *2^32-1*    (- *2^32*  1))
 (defconst *2^32-2*    (- *2^32*  2))
 (defconst *2^32-3*    (- *2^32*  3))
@@ -121,9 +123,14 @@
 ;; Group 4:
 (defconst *addr-size-override*    #x67)
 
+;; SIMD Prefixes:
 (defconst *mandatory-66h*         #x66)
 (defconst *mandatory-f2h*         #xF2)
 (defconst *mandatory-f3h*         #xF3)
+
+;; VEX Prefix:
+(defconst *vex2-byte0*            #xC5) ;; First byte of the 2-byte VEX prefix
+(defconst *vex3-byte0*            #xC4) ;; First byte of the 3-byte VEX prefix
 
 ;; ======================================================================
 
@@ -287,10 +294,13 @@
         *mxcsr-reserved*))
 
 
-;; Access GPR or XMM:
+;; Access GPR, XMM, YMM, or ZMM:
 
-(defconst *gpr-access* 0)
-(defconst *xmm-access* 1)
+(defconst *gpr-access*     0)
+(defconst *xmm-access*     1) ;; Non-VEX Encoded SIMD Instructions
+(defconst *vex-xmm-access* 2)
+(defconst *ymm-access*     3)
+(defconst *zmm-access*     4)
 
 ;; Rounding Control bit definitions (Intel manual, Mar'17, Vol. 1, Table 4-8):
 
@@ -598,7 +608,38 @@
 
      ,(b* ((lst (gl-int 0 1 16))
            (len  (len lst)))
-          (cons 'mv (append lst (list len))))))
+        (cons 'mv (append lst (list len))))))
+
+(defun define-ymm-registers ()
+  ;; 256-bit registers
+
+  `(defconsts (*YMM0* *YMM1* *YMM2* *YMM3* *YMM4* *YMM5* *YMM6* *YMM7*
+                      *YMM8* *YMM9* *YMM10* *YMM11*
+                      *YMM12* *YMM13* *YMM14* *YMM15*
+                      *ymm-register-names-len*)
+
+     ,(b* ((lst (gl-int 0 1 16))
+           (len  (len lst)))
+        (cons 'mv (append lst (list len))))))
+
+(defun define-zmm-registers ()
+  ;; 512-bit registers
+
+  `(progn
+     ;; mv can't be given more than 32 arguments, so I've had to
+     ;; separately define *zmm-register-names-len*.
+     (defconst *zmm-register-names-len* 32)
+     (defconsts (*ZMM0* *ZMM1* *ZMM2* *ZMM3* *ZMM4* *ZMM5* *ZMM6* *ZMM7*
+                        *ZMM8* *ZMM9* *ZMM10* *ZMM11*
+                        *ZMM12* *ZMM13* *ZMM14* *ZMM15*
+                        *ZMM16* *ZMM17* *ZMM18* *ZMM19* *ZMM20*
+                        *ZMM21* *ZMM22* *ZMM23* *ZMM24* *ZMM25*
+                        *ZMM26* *ZMM27* *ZMM28* *ZMM29* *ZMM30*
+                        *ZMM31*)
+
+       ,(b* ((lst (gl-int 0 1 31))
+             (len  (len lst)))
+          (cons 'mv (append lst (list len)))))))
 
 (defun define-model-specific-registers ()
   ;; At this point, we only model the MSRs that we need.  Remember,
@@ -675,6 +716,8 @@
 (make-event (define-fp-registers))
 (make-event (define-mmx-registers))
 (make-event (define-xmm-registers))
+(make-event (define-ymm-registers))
+(make-event (define-zmm-registers))
 (make-event (define-model-specific-registers))
 
 ;; ======================================================================
